Cleanup

SporkProofs/Inline.lean
@@ -3,67 +3,89 @@ import SporkProofs.Semantics
 import SporkProofs.WFSyntax
 import SporkProofs.WFSemantics
 
+/-!
+Defines an approach to inlining function definitions
+and proves that the result is well-formed.
+-/
+
 @[simp] def inlinedArgs (bret : Cont) (scope : Nat) (args : List Var) : List Var :=
   args ++ (List.range' scope bret.args.length).map Var.mk
 
-@[simp] def inlinedCont (B B' : BlockSigs) (bret : Cont) (scope : Nat) (c : Cont) : Cont :=
+@[simp] def Cont.inlined (c : Cont) (B B' : BlockSigs) (bret : Cont) (scope : Nat) : Cont :=
   .mk (c.b + B.length)
       (if B'[c.b]!.r.isExit then c.args else (inlinedArgs bret scope c.args))
 
-@[simp] def inlinedCode (B B': BlockSigs) (bret : Cont) (scope : Nat) : Code -> Code
+@[simp] def Code.inlined (B B': BlockSigs) (bret : Cont) (scope : Nat) : Code -> Code
   | .stmt e c =>
-    .stmt e (inlinedCode B B' bret scope.succ c)
+    .stmt e (c.inlined B B' bret scope.succ)
   | .goto bnext =>
-    .goto (inlinedCont B B' bret scope bnext)
+    .goto (bnext.inlined B B' bret scope)
   | .ite cond bthen belse =>
     .ite cond
-         (inlinedCont B B' bret scope bthen)
-         (inlinedCont B B' bret scope belse)
+         (bthen.inlined B B' bret scope)
+         (belse.inlined B B' bret scope)
   | .call h args bret' =>
-    .call h args (inlinedCont B B' bret scope bret')
+    .call h args (bret'.inlined B B' bret scope)
   | .retn args =>
     .goto (.mk bret.b (inlinedArgs bret scope args))
   | .spork bbody bspwn =>
-    .spork (inlinedCont B B' bret scope bbody)
-           (inlinedCont B B' bret scope bspwn)
+    .spork (bbody.inlined B B' bret scope)
+           (bspwn.inlined B B' bret scope)
   | .spoin bunpr bprom =>
-    .spoin (inlinedCont B B' bret scope bunpr)
-           (inlinedCont B B' bret scope bprom)
+    .spoin (bunpr.inlined B B' bret scope)
+           (bprom.inlined B B' bret scope)
 
-def extraadd (B : BlockSigs) (bret : Cont) (bsig : BlockSig) :=
+/--
+Determines the new bsig of an inlined block:
+- if the old bsig was exiting (i.e. down a spawn path), it remains the same
+- if the old bsig was returning (i.e. part of the main function body),
+  update the bsig to have the additional args stored in bret since
+  it will need to pass around those until the return, and also prepend
+  the caller's spork obligation to this block's
+-/
+def BlockSig.inlined (B : BlockSigs) (bret : Cont) (bsig : BlockSig) :=
   if bsig.r.isExit then
     bsig
   else
     .mk (bsig.Γ + bret.args.length) B[bret.b]!.r (bsig.σ ++ B[bret.b]!.σ)
 
-theorem add_exit {B bret} : {bsig : BlockSig} -> bsig.r.isExit -> extraadd B bret bsig = bsig
+theorem BlockSig.inlined_exit
+    {B bret} : {bsig : BlockSig} -> bsig.r.isExit ->
+    bsig.inlined B bret = bsig
   | ⟨_Γ, .exit _n, _σ⟩, _isexit => rfl
 
-theorem add_retn {B bret} : {bsig : BlockSig} -> bsig.r.isRetn -> extraadd B bret bsig = ⟨bsig.Γ + bret.args.length, B[bret.b]!.r, bsig.σ ++ B[bret.b]!.σ⟩
+theorem BlockSig.inlined_retn
+    {B bret} : {bsig : BlockSig} -> bsig.r.isRetn ->
+    bsig.inlined B bret = ⟨bsig.Γ + bret.args.length, B[bret.b]!.r, bsig.σ ++ B[bret.b]!.σ⟩
   | ⟨_Γ, .retn _n, _σ⟩, _isexit => rfl
 
-theorem add_σ {B bret} : {bsig : BlockSig} -> ∃ σ', (extraadd B bret bsig).σ = bsig.σ ++ σ'
-  | ⟨Γ, .exit n, σ⟩ => ⟨[], by simp[extraadd]⟩
+theorem BlockSig.inlined_σ {B bret} : {bsig : BlockSig} ->
+                           ∃ σ', (bsig.inlined B bret).σ = bsig.σ ++ σ'
+  | ⟨Γ, .exit n, σ⟩ => ⟨[], by simp[BlockSig.inlined]⟩
   | ⟨Γ, .retn n, σ⟩ => ⟨B[bret.b]!.σ, rfl⟩
 
-theorem add_σ_nil {B bret} : {bsig : BlockSig} -> bsig.σ ≠ [] -> (extraadd B bret bsig).σ ≠ []
+theorem BlockSig.inlined_σ_nil {B bret} : {bsig : BlockSig} -> bsig.σ ≠ [] ->
+                               (bsig.inlined B bret).σ ≠ []
   | ⟨Γ, .exit n, σ⟩, nn => nn
   | ⟨Γ, .retn n, σ⟩, nn => by
-    simp[extraadd]
+    simp[BlockSig.inlined]
     intro x
     contradiction
 
-theorem add_spork_comm {B bret bsig s} :
-                       (extraadd B bret bsig).spork s = extraadd B bret (bsig.spork s) :=
+theorem BlockSig.inlined_spork_comm
+    {B bret s} {bsig : BlockSig} :
+    (bsig.inlined B bret).spork s = (bsig.spork s).inlined B bret :=
   by simp[BlockSig.spork]
      cases h : bsig
      · case mk Γ r σ =>
        cases r
-       · case retn n => simp[extraadd]
+       · case retn n => simp[BlockSig.inlined]
        · case exit n => rfl
-theorem add_spoin_comm {B bret bsig} (σnn : bsig.σ ≠ []) :
-                       (extraadd B bret bsig).spoin = extraadd B bret bsig.spoin :=
-  by simp[BlockSig.spork, extraadd]
+
+theorem BlockSig.inlined_spoin_comm
+    {B bret} {bsig : BlockSig} (σnn : bsig.σ ≠ []) :
+    (bsig.inlined B bret).spoin = bsig.spoin.inlined B bret :=
+  by simp[BlockSig.spork, BlockSig.inlined]
      cases h : bsig
      · case mk Γ r σ =>
        cases req : r
@@ -73,9 +95,12 @@ theorem add_spoin_comm {B bret bsig} (σnn : bsig.σ ≠ []) :
          · case cons σh σt => simp
        · case exit n => rfl
 
-@[simp] def inlinedBlock (B B' : BlockSigs) (bret : Cont) (b : Block) : Block :=
+/-- only make changes if part of the main function body (i.e. non-exiting) -/
+@[simp] def Block.inlined (B B' : BlockSigs) (bret : Cont) (b : Block) : Block :=
   if b.bsig.r.isExit then b.offset_B B.length else
-    Block.mk (extraadd B bret b.bsig) (inlinedCode B B' bret b.bsig.Γ b.code)
+    Block.mk (b.bsig.inlined B bret) (b.code.inlined B B' bret b.bsig.Γ)
+
+def Block.inlined_ext {B B' bret} : Block.inlined B B' bret = (·.inlined B B' bret) := rfl
 
 theorem inlinedArgsRangeWF :
     (extraArity : Nat) -> (scope : Nat) ->
@@ -88,546 +113,528 @@ theorem inlinedArgsRangeWF :
            inlinedArgsRangeWF extraArity scope.succ)
 
 theorem inlinedArgsWF' (bret : Cont) {scope : Nat} : {args : List Var} ->
-                       IVec (scope ⊢ · WF-var) args -> IVec ((scope + bret.args.length) ⊢ · WF-var) args
+                       IVec (scope ⊢ · WF-var) args ->
+                       IVec ((scope + bret.args.length) ⊢ · WF-var) args
   | _args, wf => wf.weaken
 
 theorem inlinedArgsWF (bret : Cont) {scope : Nat} {args : List Var}
                       (wf : IVec (scope ⊢ · WF-var) args) :
-                      IVec ((scope + bret.args.length) ⊢ · WF-var) (inlinedArgs bret scope args) :=
+                      IVec ((scope + bret.args.length) ⊢ · WF-var)
+                           (inlinedArgs bret scope args) :=
   (inlinedArgsWF' bret wf).append (inlinedArgsRangeWF bret.args.length scope)
 
-theorem inlinedContWFRets
+theorem Cont.WFRets.inlined
         {B B' bsig rets} {bret c : Cont}
         (wf : B'; bsig ⊢ c(rets) WF-cont) :
-        (B ++ B'.map (extraadd B bret)); (extraadd B bret bsig) ⊢ (inlinedCont B B' bret bsig.Γ c)(rets) WF-cont :=
+        (B ++ B'.map (·.inlined B bret));
+          (bsig.inlined B bret) ⊢ (c.inlined B B' bret bsig.Γ)(rets) WF-cont :=
   match bsig with
     | ⟨Γ, .exit n, σ⟩ =>
-      let h := congrArg BlockSig.r wf.bsig
+      have h := congrArg BlockSig.r wf.bsig
       by simp at h
          exact
       .mk (by simp[Nat.add_comm B.length, getElem!_pos B' c.b wf.blt, h]
               exact wf.blt)
           (by simp[-List.getElem!_eq_getElem?_getD, getElem!_pos B' c.b wf.blt, h]
-              show extraadd B bret (B'[c.b]'wf.blt) =
+              show (B'[c.b]'wf.blt).inlined B bret =
                    BlockSig.mk (c.args.length + rets) (ResultSig.exit n) σ
-              rw[add_exit (by rw[h]; rfl)]
+              rw[(B'[c.b]'wf.blt).inlined_exit (by rw[h]; rfl)]
               exact wf.bsig)
           (by simpa[getElem!_pos B' c.b wf.blt, h] using wf.args)
     | ⟨Γ, .retn n, σ⟩ =>
       .mk (by simp[Nat.add_comm c.b B.length, wf.blt])
           (by simp[-List.getElem!_eq_getElem?_getD,
                    getElem!_pos B' c.b wf.blt, wf.bsig,
-                   Nat.add_comm c.b B.length, extraadd]
+                   Nat.add_comm c.b B.length, BlockSig.inlined]
               rw[Nat.add_assoc, Nat.add_comm rets bret.args.length, ← Nat.add_assoc])
-          (by simpa[getElem!_pos B' c.b wf.blt, wf.bsig, extraadd]
+          (by simpa[getElem!_pos B' c.b wf.blt, wf.bsig, BlockSig.inlined]
               using inlinedArgsWF bret wf.args)
 
-theorem inlinedContWF
+theorem Cont.WF.inlined
         {B B' bsig} {bret c : Cont}
         (wf : B'; bsig ⊢ c WF-cont) :
-        (B ++ B'.map (extraadd B bret)); (extraadd B bret bsig) ⊢ (inlinedCont B B' bret bsig.Γ c) WF-cont :=
-  (inlinedContWFRets wf.cast0).cast0
+        (B ++ B'.map (·.inlined B bret));
+          (bsig.inlined B bret) ⊢ (c.inlined B B' bret bsig.Γ) WF-cont :=
+  wf.cast0.inlined.cast0
 
-theorem inlinedContExit {B B' : BlockSigs} {bret scope} {c : Cont}
-                        (isexit : B'[c.b]!.r.isExit) :
-                        inlinedCont B B' bret scope c = c.offset_B B.length :=
-  by simp[Cont.offset_B, -List.getElem!_eq_getElem?_getD, -ResultSig.isExit]
-     intro isexitfalse
-     rw[isexitfalse] at isexit
-     contradiction
+-- theorem Cont.inlined_exit {B B' : BlockSigs} {bret scope} {c : Cont}
+--                           (isexit : B'[c.b]!.r.isExit) :
+--                           c.inlined B B' bret scope = c.offset_B B.length :=
+--   by simp[Cont.offset_B, -List.getElem!_eq_getElem?_getD, -ResultSig.isExit]
+--      intro isexitfalse
+--      rw[isexitfalse] at isexit
+--      contradiction
 
-theorem inlinedContMapWFRets {B B' : BlockSigs} {bsig : BlockSig} {c rets bret}
-                             (isexit : bsig.r.isExit) (wf : B'; bsig ⊢ c(rets) WF-cont) :
-                             (B'.map (extraadd B bret)); (extraadd B bret bsig) ⊢ c(rets) WF-cont :=
-  (add_exit isexit).symm ▸
-  .mk ((List.length_map (extraadd B bret)).symm ▸ wf.blt)
+--inlinedContMapWFRets
+theorem Cont.WFRets.inlined_map
+    {B B' : BlockSigs} {bsig : BlockSig} {c rets bret}
+    (isexit : bsig.r.isExit) (wf : B'; bsig ⊢ c(rets) WF-cont) :
+    (B'.map (·.inlined B bret)); (bsig.inlined B bret) ⊢ c(rets) WF-cont :=
+  (bsig.inlined_exit isexit).symm ▸
+  .mk ((List.length_map (BlockSig.inlined B bret)).symm ▸ wf.blt)
       (wf.bsig ▸
-       List.getElem_map (extraadd B bret) ▸
-       add_exit (wf.bsig ▸ isexit))
+       List.getElem_map (BlockSig.inlined B bret) ▸
+       BlockSig.inlined_exit (wf.bsig ▸ isexit))
       wf.args
 
-theorem inlinedContMapWF {B B' : BlockSigs} {bsig : BlockSig} {c bret}
-                         (isexit : bsig.r.isExit) (wf : B'; bsig ⊢ c WF-cont) :
-                         (B'.map (extraadd B bret)); (extraadd B bret bsig) ⊢ c WF-cont :=
-  (inlinedContMapWFRets isexit wf.cast0).cast0
+theorem Cont.WF.inlined_map
+    {B B' : BlockSigs} {bsig : BlockSig} {c bret}
+    (isexit : bsig.r.isExit) (wf : B'; bsig ⊢ c WF-cont) :
+    (B'.map (·.inlined B bret)); (bsig.inlined B bret) ⊢ c WF-cont :=
+  (wf.cast0.inlined_map isexit).cast0
 
-@[simp] theorem inlinedContb {B B' bret scope c} :
-                             (inlinedCont B B' bret scope c).b = c.b + B.length :=
+@[simp] theorem Cont.inlined_b {B B' bret scope} {c : Cont} :
+                               (c.inlined B B' bret scope).b = c.b + B.length :=
   rfl
 
-theorem expand_bsig_retn : {bsig : BlockSig} ->
-                           bsig.r.isRetn -> bsig = ⟨bsig.Γ, .retn bsig.r.n, bsig.σ⟩
+theorem BlockSig.expand_retn :
+    {bsig : BlockSig} -> bsig.r.isRetn -> bsig = ⟨bsig.Γ, .retn bsig.r.n, bsig.σ⟩
   | ⟨_Γ, .retn _n, _σ⟩, _isretn => rfl
-theorem expand_bsig_exit : {bsig : BlockSig} -> bsig.r.isExit ->
-                           bsig = ⟨bsig.Γ, .exit bsig.r.n, bsig.σ⟩
+theorem BlockSig.expand_exit :
+    {bsig : BlockSig} -> bsig.r.isExit -> bsig = ⟨bsig.Γ, .exit bsig.r.n, bsig.σ⟩
   | ⟨_Γ, .exit _n, _σ⟩, _isretn => rfl
-theorem expand_list {α} : {l : List α} -> (nn : l ≠ []) -> l = l.head nn :: l.tail
+
+theorem List.expand {α} : {l : List α} -> (nn : l ≠ []) -> l = l.head nn :: l.tail
   | _h :: _t, _nn => rfl
-theorem List.head!_eq_head {α} [Inhabited α] : {l : List α} -> (nn : l ≠ []) -> l.head nn = l.head!
+theorem List.head!_eq_head {α} [Inhabited α] : {l : List α} -> (nn : l ≠ []) ->
+                           l.head nn = l.head!
   | _h :: _t, _nn => rfl
 
-theorem inlinedCodeWF
+theorem Code.WF.inlined
     {fsigs B B' bsig bretsigΓ}
-    -- (extra : Extra)
     (bret : Cont)
     (isretn : bsig.r.isRetn)
     (bretwf : B; ⟨bretsigΓ, B[bret.b]!.r, B[bret.b]!.σ⟩ ⊢ bret(bsig.r.n) WF-cont) :
-    -- (bretlt : bret < B.length)
-    -- (bretsig : B[bret] = ⟨bsig.r.n + extra.Γ, bsig.r, extra.σ⟩)
---    (bretsig : (B[bret].Γ = bsig.r + extra.Γ) ∧ (B[bret].r = bsig.r) ∧ (B[bret].σ = extra.σ))
-    -- (bslen : B.length = extra.offset)
-    -- (req : extra.r = bsig.r) :
     {c : Code} ->
     fsigs; B'; bsig ⊢ c WF-code ->
-    fsigs; (B ++ B'.map (extraadd B bret)); (extraadd B bret bsig) ⊢
-      (inlinedCode B B' bret bsig.Γ c) WF-code
+    fsigs; (B ++ B'.map (·.inlined B bret)); (bsig.inlined B bret) ⊢
+      (c.inlined B B' bret bsig.Γ) WF-code
   | .stmt e c, wf =>
-    let z := inlinedCodeWF (bsig := bsig.bind) bret isretn bretwf wf.stmt_code
-    expand_bsig_retn isretn ▸
+    have z := wf.stmt_code.inlined (bsig := bsig.bind) bret isretn bretwf
+    BlockSig.expand_retn isretn ▸
     .stmt wf.stmt_expr.weaken
-          (by rw[expand_bsig_retn isretn] at z
-              simpa[Nat.add_right_comm, extraadd] using z)
+          (by rw[BlockSig.expand_retn isretn] at z
+              simpa[Nat.add_right_comm, BlockSig.inlined] using z)
   | .goto bnext, wf =>
-    .goto (inlinedContWF wf.goto_bnext)
+    .goto wf.goto_bnext.inlined
   | .ite cond bthen belse, wf =>
-    .ite (expand_bsig_retn isretn ▸ wf.ite_cond.weaken)
-         (inlinedContWF wf.ite_bthen)
-         (inlinedContWF wf.ite_belse)
+    .ite (BlockSig.expand_retn isretn ▸ wf.ite_cond.weaken)
+         wf.ite_bthen.inlined
+         wf.ite_belse.inlined
   | .call h args bret', wf =>
     .call wf.call_flt
-          (wf.call_arity)
-          (expand_bsig_retn isretn ▸ inlinedArgsWF' bret wf.call_args)
-          (inlinedContWFRets wf.call_bret)
+          wf.call_arity
+          (BlockSig.expand_retn isretn ▸ inlinedArgsWF' bret wf.call_args)
+          wf.call_bret.inlined
   | .retn args, .retn len sn_nil argswf =>
-    expand_bsig_retn isretn ▸
+    BlockSig.expand_retn isretn ▸
     .goto (.mk (by simp[Nat.lt_add_right B'.length bretwf.blt])
-               (by rw[extraadd]
+               (by rw[BlockSig.inlined]
                    simp only [getters]
                    rw[List.getElem_append_left bretwf.blt]
-                   --simp only [getters]
-                   --rw[← len]
                    rw[sn_nil]
-                   let x := bretwf.bsig
+                   have x := bretwf.bsig
                    rw (occs := [2]) [len] at x
                    rw[x]
-                   simp[Nat.add_comm]
-                   
-                   )
+                   simp[Nat.add_comm])
                (inlinedArgsWF bret argswf))
   | .spork bbody bspwn, wf =>
-    let bspwnexit : (B'[bspwn.b]'wf.spork_bspwn.blt).r.isExit = true :=
+    have bspwnexit : (B'[bspwn.b]'wf.spork_bspwn.blt).r.isExit = true :=
       congrArg BlockSig.r wf.spork_bspwn.bsig ▸
       getElem!_pos B' bspwn.b wf.spork_bspwn.blt ▸
       by simp[BlockSig.spwn]
-    .spork (inlinedContb ▸
-            by --simp only [extraadd.eq_1]
-               --simp only [getters]
-               rw[getElem!_pos (B ++ B'.map (extraadd B bret)) (bspwn.b + B.length)
+    .spork (Cont.inlined_b ▸
+            by rw[getElem!_pos (B ++ B'.map (·.inlined B bret)) (bspwn.b + B.length)
                      (by simp[Nat.add_comm bspwn.b B.length]
-                         exact wf.spork_bspwn.blt)]
-               rw[← List.getElem_append_right' (l₁ := B)
-                      (l₂ := B'.map (extraadd B bret))
-                      (List.length_map (as := B') (extraadd B bret) ▸
-                       wf.spork_bspwn.blt)]
-               rw[List.getElem_map]
-               let x := congrArg BlockSig.r wf.spork_bspwn.bsig
+                         exact wf.spork_bspwn.blt),
+                  ← List.getElem_append_right' (l₁ := B)
+                      (l₂ := B'.map (·.inlined B bret))
+                      (List.length_map (as := B') (BlockSig.inlined B bret) ▸
+                       wf.spork_bspwn.blt),
+                  List.getElem_map]
+               have x := congrArg BlockSig.r wf.spork_bspwn.bsig
                simp only [getters, BlockSig.spwn] at x
-               rw[@expand_bsig_exit (B'[bspwn.b]'wf.spork_bspwn.blt) (x ▸ rfl)]
+               rw[(B'[bspwn.b]'wf.spork_bspwn.blt).expand_exit (x ▸ rfl)]
                rw[x]
-               simp[extraadd])
-           (add_spork_comm ▸
-            inlinedContWF
-              (by rw[inlinedContb,
-                     getElem!_pos (B ++ B'.map (extraadd B bret)) (bspwn.b + B.length)
+               simp[BlockSig.inlined])
+           (BlockSig.inlined_spork_comm ▸
+            Cont.WF.inlined
+              (by rw[Cont.inlined_b,
+                     getElem!_pos (B ++ B'.map (·.inlined B bret)) (bspwn.b + B.length)
                        (by simp[Nat.add_comm bspwn.b B.length]
                            exact wf.spork_bspwn.blt),
-                     ← List.getElem_append_right' (l₁ := B) (l₂ := B'.map (extraadd B bret))
-                         (i := bspwn.b) (List.length_map (as := B') (extraadd B bret) ▸
+                     ← List.getElem_append_right' (l₁ := B) (l₂ := B'.map (·.inlined B bret))
+                         (i := bspwn.b) (List.length_map (as := B') (·.inlined B bret) ▸
                                          wf.spork_bspwn.blt)]
-                  let h : ((B'.map (extraadd B bret))[bspwn.b]'
-                             (B'.length_map (extraadd B bret) ▸ wf.spork_bspwn.blt)).r =
+                  have h : ((B'.map (BlockSig.inlined B bret))[bspwn.b]'
+                             (B'.length_map (·.inlined B bret) ▸ wf.spork_bspwn.blt)).r =
                           B'[bspwn.b]!.r :=
-                    List.getElem_map (extraadd B bret) ▸
-                    let y := wf.spork_bspwn.bsig
-                    by rw[add_exit bspwnexit]
+                    List.getElem_map (BlockSig.inlined B bret) ▸
+                    have y := wf.spork_bspwn.bsig
+                    by rw[BlockSig.inlined_exit bspwnexit]
                        rw[← getElem!_pos B' bspwn.b wf.spork_bspwn.blt]
                   rw[h]
                   exact wf.spork_bbody))
-           (let y := inlinedContWF wf.spork_bspwn
+           (have y := wf.spork_bspwn.inlined
             by rw[BlockSig.spwn,
-                  inlinedContb,
-                  getElem!_pos (B ++ B'.map (extraadd B bret)) (bspwn.b + B.length)
+                  Cont.inlined_b,
+                  getElem!_pos (B ++ B'.map (·.inlined B bret)) (bspwn.b + B.length)
                     (by simpa[Nat.add_comm bspwn.b B.length]
                         using wf.spork_bspwn.blt),
                   ← List.getElem_append_right' B _,
-                  List.getElem_map (extraadd B bret)
-                    (h := (List.length_map (extraadd B bret)).symm ▸ wf.spork_bspwn.blt),
-                  add_exit bspwnexit]               
+                  List.getElem_map (BlockSig.inlined B bret)
+                    (h := (List.length_map (BlockSig.inlined B bret)).symm ▸
+                          wf.spork_bspwn.blt),
+                  BlockSig.inlined_exit bspwnexit]
                rw[BlockSig.spwn,
-                  add_exit rfl,
+                  BlockSig.inlined_exit rfl,
                   getElem!_pos B' bspwn.b wf.spork_bspwn.blt] at y
                simp only [getters] at y
-               rw[add_retn isretn]
+               rw[BlockSig.inlined_retn isretn]
                exact y.weaken_Γ)
   | .spoin bunpr bprom, wf =>
-    .spoin (λ x => by rw[add_retn isretn] at x
+    .spoin (λ x => by rw[BlockSig.inlined_retn isretn] at x
                       simp at x
                       exact wf.spoin_oblg x.1)
-           (add_spoin_comm wf.spoin_oblg ▸
-            inlinedContWF wf.spoin_bunpr)
-           (let x : bsig.spoin.Γ = bsig.Γ := rfl
-            let ⟨σ', σ_σ'⟩ := add_σ (B := B) (bret := bret) (bsig := bsig)
-            let y : bsig.σ.head wf.spoin_oblg =
-                    (extraadd B bret bsig).σ.head (add_σ_nil wf.spoin_oblg) :=
+           (BlockSig.inlined_spoin_comm wf.spoin_oblg ▸
+            wf.spoin_bunpr.inlined)
+           (have ⟨σ', σ_σ'⟩ := BlockSig.inlined_σ (B := B) (bret := bret) (bsig := bsig)
+            have y : bsig.σ.head wf.spoin_oblg =
+                    (bsig.inlined B bret).σ.head (BlockSig.inlined_σ_nil wf.spoin_oblg) :=
               List.head!_eq_head wf.spoin_oblg ▸
-              List.head!_eq_head (add_σ_nil wf.spoin_oblg) ▸
+              List.head!_eq_head (BlockSig.inlined_σ_nil wf.spoin_oblg) ▸
               σ_σ' ▸
-              expand_list wf.spoin_oblg ▸
+              List.expand wf.spoin_oblg ▸
               rfl
             y ▸
-            add_spoin_comm wf.spoin_oblg ▸
-            x ▸
-            inlinedContWFRets wf.spoin_bprom)
+            BlockSig.inlined_spoin_comm wf.spoin_oblg ▸
+            wf.spoin_bprom.inlined)
 
-theorem offsetCodeWF
+theorem Code.WF.inlined_offset
     {fsigs B B' bret bsig}
     (isexit : bsig.r.isExit) :
     {c : Code} ->
     fsigs; B'; bsig ⊢ c WF-code ->
-    fsigs; (B ++ B'.map (extraadd B bret)); (extraadd B bret bsig) ⊢
+    fsigs; (B ++ B'.map (·.inlined B bret)); (bsig.inlined B bret) ⊢
       (c.offset_B B.length) WF-code
   | .stmt e c, wf =>
-    .stmt ((add_exit isexit).symm ▸ wf.stmt_expr)
-          (let x := offsetCodeWF (bsig := bsig.bind) isexit wf.stmt_code
-           by rw[@add_exit B bret bsig isexit]
-              rw[@add_exit B bret bsig.bind isexit] at x
+    .stmt ((BlockSig.inlined_exit isexit).symm ▸ wf.stmt_expr)
+          (have x := wf.stmt_code.inlined_offset (bsig := bsig.bind) isexit
+           by rw[bsig.inlined_exit isexit]
+              rw[bsig.bind.inlined_exit isexit] at x
               exact x)
   | .goto bnext, wf =>
-    .goto (inlinedContMapWF isexit wf.goto_bnext).weaken_Bᵣ
+    .goto (wf.goto_bnext.inlined_map isexit).weaken_Bᵣ
   | .ite cond bthen belse, wf =>
-    .ite ((add_exit isexit).symm ▸ wf.ite_cond)
-         (inlinedContMapWF isexit wf.ite_bthen).weaken_Bᵣ
-         (inlinedContMapWF isexit wf.ite_belse).weaken_Bᵣ
+    .ite ((BlockSig.inlined_exit isexit).symm ▸ wf.ite_cond)
+         (wf.ite_bthen.inlined_map isexit).weaken_Bᵣ
+         (wf.ite_belse.inlined_map isexit).weaken_Bᵣ
   | .call h args bret', wf =>
     .call wf.call_flt
           wf.call_arity
-          ((add_exit isexit).symm ▸ wf.call_args)
-          (inlinedContMapWFRets isexit wf.call_bret).weaken_Bᵣ
+          ((BlockSig.inlined_exit isexit).symm ▸ wf.call_args)
+          (wf.call_bret.inlined_map isexit).weaken_Bᵣ
   | .retn args, wf =>
-    (add_exit isexit).symm ▸ 
+    (BlockSig.inlined_exit isexit).symm ▸
     .retn wf.retn_length wf.retn_oblg wf.retn_args
   | .spork bbody bspwn, wf =>
-    (add_exit isexit).symm ▸
-    let bspwnlt : bspwn.b < B'.length :=
+    (BlockSig.inlined_exit isexit).symm ▸
+    have bspwnlt : bspwn.b < B'.length :=
       wf.spork_bspwn.blt
-    let x : (B ++ B'.map (extraadd B bret))[(Cont.offset_B (List.length B) bspwn).b]! =
-            (B'.map (extraadd B bret))[bspwn.b]! :=
-      Cont.offset_B_b ▸
-      getElem!_pos (B ++ B'.map (extraadd B bret)) (bspwn.b + B.length)
+    have x : (B ++ B'.map (·.inlined B bret))[(bspwn.offset_B (List.length B)).b]! =
+            (B'.map (·.inlined B bret))[bspwn.b]! :=
+      bspwn.offset_B_b ▸
+      getElem!_pos (B ++ B'.map (·.inlined B bret)) (bspwn.b + B.length)
         (List.length_append ▸
          Nat.add_comm bspwn.b B.length ▸
          Nat.add_lt_add_iff_left.mpr
-           ((List.length_map (extraadd B bret)).symm ▸ bspwnlt)) ▸
-      List.getElem_append_right' B (List.length_map (extraadd B bret) ▸ bspwnlt) ▸
-      (getElem!_pos (B'.map (extraadd B bret)) bspwn.b
-        ((List.length_map (extraadd B bret)).symm ▸ bspwnlt)).symm
-    let y : (B'.map (extraadd B bret))[bspwn.b]! = B'[bspwn.b]! :=
-      getElem!_pos (B'.map (extraadd B bret)) bspwn.b
-        ((List.length_map (extraadd B bret)).symm ▸ bspwnlt) ▸
+           ((List.length_map (BlockSig.inlined B bret)).symm ▸ bspwnlt)) ▸
+      List.getElem_append_right' B (List.length_map (BlockSig.inlined B bret) ▸ bspwnlt) ▸
+      (getElem!_pos (B'.map (·.inlined B bret)) bspwn.b
+        ((List.length_map (BlockSig.inlined B bret)).symm ▸ bspwnlt)).symm
+    have y : (B'.map (·.inlined B bret))[bspwn.b]! = B'[bspwn.b]! :=
+      getElem!_pos (B'.map (·.inlined B bret)) bspwn.b
+        ((List.length_map (BlockSig.inlined B bret)).symm ▸ bspwnlt) ▸
       getElem!_pos B' bspwn.b bspwnlt ▸
-      List.getElem_map (extraadd B bret) ▸
-      add_exit (bsig := B'[bspwn.b])
+      List.getElem_map (BlockSig.inlined B bret) ▸
+      --BlockSig.inlined_exit (bsig := B'[bspwn.b])
+      B'[bspwn.b].inlined_exit
         (getElem!_pos B' bspwn.b bspwnlt ▸ wf.spork_exit)
     .spork (x ▸ y ▸ wf.spork_exit)
-           (x ▸ add_exit (bsig := bsig.spork (B'.map (extraadd B bret))[bspwn.b]!.r.n) isexit ▸
-           (inlinedContMapWF (bsig := bsig.spork (B'.map (extraadd B bret))[bspwn.b]!.r.n) isexit
-             (y ▸ wf.spork_bbody)).weaken_Bᵣ)
-           (x ▸ add_exit (bsig := bsig.spwn (B'.map (extraadd B bret))[bspwn.b]!.r.n) rfl ▸
-             (inlinedContMapWF (bsig := bsig.spwn (B'.map (extraadd B bret))[bspwn.b]!.r.n)
-               rfl (y ▸ wf.spork_bspwn)).weaken_Bᵣ)
+           (x ▸
+            (bsig.spork (B'.map (BlockSig.inlined B bret))[bspwn.b]!.r.n).inlined_exit isexit ▸
+            ((y ▸ wf.spork_bbody).inlined_map
+                (bsig := bsig.spork (B'.map (BlockSig.inlined B bret))[bspwn.b]!.r.n)
+                isexit).weaken_Bᵣ)
+           (x ▸ (bsig.spwn (B'.map (BlockSig.inlined B bret))[bspwn.b]!.r.n).inlined_exit rfl ▸
+             ((y ▸ wf.spork_bspwn).inlined_map
+                (bsig := bsig.spwn (B'.map (BlockSig.inlined B bret))[bspwn.b]!.r.n)
+                rfl).weaken_Bᵣ)
   | .spoin bunpr bprom, wf =>
-    (add_exit isexit).symm ▸ 
-    .spoin (wf.spoin_oblg)
-           (add_exit (bsig := bsig.spoin) isexit ▸
-            (inlinedContMapWF (bsig := bsig.spoin) isexit wf.spoin_bunpr).weaken_Bᵣ)
-           (add_exit (bsig := bsig.spoin) isexit ▸
-            (inlinedContMapWFRets (bsig := bsig.spoin) isexit wf.spoin_bprom).weaken_Bᵣ)
+    (BlockSig.inlined_exit isexit).symm ▸
+    .spoin wf.spoin_oblg
+           (bsig.spoin.inlined_exit isexit ▸
+            (wf.spoin_bunpr.inlined_map (bsig := bsig.spoin) isexit).weaken_Bᵣ)
+           (bsig.spoin.inlined_exit isexit ▸
+            (wf.spoin_bprom.inlined_map (bsig := bsig.spoin) isexit).weaken_Bᵣ)
 
-theorem inlinedBlockWF
+theorem Block.WF.inlined
     {fsigs B B' bret b bretsigΓ}
     (bretwf : B; ⟨bretsigΓ, B[bret.b]!.r, B[bret.b]!.σ⟩ ⊢ bret(b.bsig.r.n) WF-cont)
     (wf : fsigs; B' ⊢ b WF-block) :
-    fsigs; (B ++ B'.map (extraadd B bret)) ⊢ (inlinedBlock B B' bret b) WF-block :=
+    fsigs; (B ++ B'.map (·.inlined B bret)) ⊢ (b.inlined B B' bret) WF-block :=
   if isexit : b.bsig.r.isExit then
-    by rw[inlinedBlock, isexit]
+    by rw[Block.inlined, isexit]
        simp only [↓reduceIte]
        apply Block.WF.mk
        simp only [Block.offset_B, getters]
-       let x := offsetCodeWF (B := B) (bret := bret) isexit wf.code
-       rw[add_exit isexit] at x
+       have x := wf.code.inlined_offset (B := B) (bret := bret) isexit
+       rw[BlockSig.inlined_exit isexit] at x
        exact x
   else
-    let isretn : b.bsig.r.isRetn := b.bsig.r.not_isExit_isRetn isexit
-    .mk (by simp only [inlinedBlock, Block.offset_B, isexit,
+    have isretn : b.bsig.r.isRetn := b.bsig.r.not_isExit_isRetn isexit
+    .mk (by simp only [Block.inlined, Block.offset_B, isexit,
                        Bool.false_eq_true, reduceIte, getters]
-            exact inlinedCodeWF bret isretn bretwf wf.code)
+            exact wf.code.inlined bret isretn bretwf)
 
-@[simp] def inlinedFuncBody (B : BlockSigs) (g : Func) (bret : Cont) : List Block :=
-  g.blocks.map (inlinedBlock B g.B bret)
+@[simp] def Func.inlined_body (B : BlockSigs) (g : Func) (bret : Cont) : List Block :=
+  g.blocks.map (·.inlined B g.B bret)
 
-theorem inlinedFuncBodyWF
+theorem Func.WF.inlined_body
           {fsigs B g bret bretsigΓ}
           (bretwf : B; ⟨bretsigΓ, B[bret.b]!.r, B[bret.b]!.σ⟩ ⊢ bret(g.fsig.ret) WF-cont)
           (wf : fsigs ⊢ g WF-func) :
-          IVec (λ b => (fsigs; (B ++ g.B.map (extraadd B bret)) ⊢ b WF-block) /- ∧
-                       (B[bret.b]!.r.isRetn -> b.bsig.r.isRetn -> b.bsig.r = B[bret.b]!.r)-/)
-               (inlinedFuncBody B g bret) :=
-  let bretlt : bret.b < B.length :=
+          IVec (λ b => (fsigs; (B ++ g.B.map (·.inlined B bret)) ⊢ b WF-block))
+               (g.inlined_body B bret) :=
+  have bretlt : bret.b < B.length :=
     bretwf.blt
-  let x : B[bret.b]! = B[bret.b] :=
+  have x : B[bret.b]! = B[bret.b] :=
     getElem!_pos B bret.b bretlt
-  let Γeq : bret.args.length + g.fsig.ret = B[bret.b].Γ :=
+  have Γeq : bret.args.length + g.fsig.ret = B[bret.b].Γ :=
     by simpa only [getters] using congrArg BlockSig.Γ bretwf.bsig.symm
   by simpa[← x, -List.getElem!_eq_getElem?_getD] using
     (wf.blocks.zip wf.retns).from_map'
-      (inlinedBlock B g.B bret)
+      (·.inlined B g.B bret)
       λ (b : Block) ⟨wf', req'⟩ =>
         if isexit : b.bsig.r.isExit then
-          by rw[inlinedBlock, isexit]
-             --apply And.intro
-             · apply Block.WF.mk
-               simpa[add_exit isexit]
-               using offsetCodeWF isexit wf'.code
-             -- · intro bretisretn isretn
-             --   cases h : b.bsig.r <;>
-             --   (simp at isretn isexit
-             --    rw[h] at isretn isexit
-             --    contradiction)
+          by simp only
+             rw[Block.inlined, isexit]
+             apply Block.WF.mk
+             simpa[BlockSig.inlined_exit isexit]
+             using wf'.code.inlined_offset isexit
         else by
-          let isretn := ResultSig.not_isExit_isRetn isexit
-          -- apply And.intro
-          · simpa[x]
-            using @inlinedBlockWF fsigs B g.B bret b bretsigΓ (req' isretn ▸ bretwf) wf'
-          -- · intro bretisretn _
-          --   simp only [inlinedBlock]
-          --   rw[(Bool.not_eq_not (b := false)).mp isexit]
-          --   simp only [Bool.false_eq_true, reduceIte, getters]
-          --   rw[add_retn isretn]
-          --   simp only [getters]
+          have isretn := ResultSig.not_isExit_isRetn isexit
+          simpa[x]
+          using @wf'.inlined fsigs B g.B bret b bretsigΓ (req' isretn ▸ bretwf)
 
-@[simp] def replaceCallInCode (g : FuncIdx) (offset : Nat) (c : Code) : Option (Code × Cont) :=
-  let (e, ⟨t, _p⟩) := c.split
-  match t with
-    | .call h args bret =>
-      if h = g then
-        some (Code.merge e (Code.goto (.mk offset (args ++ bret.args))), bret)
-      else
-        none
-    | _ => none
-
-
-@[simp] def inlinedFuncH (g : Func) (gidx : FuncIdx) :
-                 List Block -> List Block -> List Block -> List Block
+@[simp] def Func.inlined_h
+    (g : Func) (gidx : FuncIdx) :
+    List Block -> List Block -> List Block -> List Block
   | bacc, [], gacc => bacc ++ gacc
   | bacc, .mk bsig c :: bs, gacc =>
-    let (b', gacc') :=
-      (replaceCallInCode gidx
-          (bacc ++ [Block.mk bsig c] ++ bs ++ gacc).length c).elim
-        (.mk bsig c, [])
-        (λ (c', bret) =>
+    let (b', gacc') := match c.split with
+      | (e, ⟨.call h args bret, _notstmt⟩) =>
+        if h = gidx then
+          let B := bacc ++ [Block.mk bsig c] ++ bs ++ gacc
+          let c' := Code.merge e (Code.goto (.mk B.length (args ++ bret.args)))
           (.mk bsig c',
-           inlinedFuncBody ((bacc ++ [Block.mk bsig c'] ++ bs ++ gacc).map Block.bsig) g bret))
-    inlinedFuncH g gidx (bacc ++ [b']) bs (gacc ++ gacc')
+           g.inlined_body (B.map Block.bsig) bret)
+        else
+          (.mk bsig c, [])
+      | _ => (.mk bsig c, [])
+    g.inlined_h gidx (bacc ++ [b']) bs (gacc ++ gacc')
 
-theorem inlinedFuncHWF
+
+theorem Func.WF.inlined_h
         {fsigs fsig g gidx bacc gacc} :
         {bs : List Block} ->
         fsigs ⊢ g WF-func ->
         (_ : gidx < fsigs.length) ->
         fsigs[gidx] = g.fsig ->
         fsigs ⊢ Func.mk fsig (bacc ++ bs ++ gacc) WF-func ->
-        fsigs ⊢ Func.mk fsig (inlinedFuncH g gidx bacc bs gacc) WF-func
+        fsigs ⊢ Func.mk fsig (g.inlined_h gidx bacc bs gacc) WF-func
   | [], gwf, glt, gsig, wf => List.append_nil bacc ▸ wf
   | .mk bsig c :: bs, gwf, glt, gsig, wf => by
     simp
     match cspliteq : c.split with
-      | (es, ⟨t, t_neq_stmt⟩) =>
-        cases t <;> simp <;> try (apply inlinedFuncHWF gwf glt gsig; simpa using wf)
-        · case call h args bret =>
-          if heqg : h ≠ gidx then
-            simp[heqg]
-            apply inlinedFuncHWF gwf glt gsig
-            simpa using wf
-          else
-            have heqg := Decidable.of_not_not heqg
-            rw[heqg]
-            simp[heqg] at cspliteq
-            simp
-            let c' : Code :=
-              .merge es (.goto (.mk (bacc.length + (bs.length + gacc.length + 1))
-                                   (args ++ bret.args)))
-            let gacc' := inlinedFuncBody ((bacc ++ [Block.mk bsig c'] ++ bs ++ gacc).map
-                                            Block.bsig) g bret
-            let B := (bacc ++ Block.mk bsig c' :: bs ++ gacc ++ gacc').map (·.bsig)
-            have wf' := wf.blocks.get ⟨bacc.length, by simp⟩
-            simp at wf'
-            have cwf := wf'.code
-            have splitwf := Code.WF.split_wf cwf
-            simp[cspliteq] at splitwf
-            have c'wf : fsigs; B; bsig ⊢ c' WF-code := by
-              simp[c', B]
-              apply Code.WF.merge_wf
-              · exact λ ⟨i, il⟩ => splitwf.1 ⟨i, by simp_all⟩
-              · apply Code.WF.goto
-                apply Cont.WF.mk <;> simp
-                · simp[gacc']
-                  have gh := gwf.head.get0eq
-                  simp at gh; rw[gh]; simp[extraadd, -List.getElem!_eq_getElem?_getD]
-                  have req := congrArg BlockSig.r splitwf.2.call_bret.bsig
-                  have σeq := congrArg BlockSig.σ splitwf.2.call_bret.bsig
-                  rw[getElem!_pos _ bret.b splitwf.2.call_bret.blt]
-                  exact gsig ▸ ⟨splitwf.2.call_arity, req, σeq⟩
-                · exact splitwf.2.call_args.append splitwf.2.call_bret.args
-                · match gacc'eq : gacc' with
-                    | [] => simp[gacc'] at gacc'eq
-                            simpa[gacc'eq] using gwf.head.headtail
-                    | _ :: _ => simp
-            have b'wf : fsigs; B ⊢ ⟨bsig, c'⟩ WF-block := .mk c'wf
-            have wfblocks := wf.blocks
-            have ⟨tmp, gaccwf⟩ := wf.blocks.unappend
-            have ⟨baccwf, tmp'⟩ := tmp.unappend
-            have bswf := tmp'.tail
-            have helper {l : List Block}
-                       (v : IVec (fsigs; ((bacc ++ Block.mk bsig c :: bs ++ gacc).map
-                                            Block.bsig) ⊢ · WF-block) l) :
-                       IVec (Block.WF fsigs ((bacc ++ [Block.mk bsig c'] ++ bs ++
-                                                   (gacc ++ gacc')).map Block.bsig)) l :=
-              v.map (λ b x => by simpa using x.weaken_Bₗ (B' := gacc'.map (·.bsig)))
-            have wf'' : fsigs ⊢ ⟨fsig, bacc ++ [.mk bsig c'] ++
-                                         bs ++ (gacc ++ gacc')⟩ WF-func := by
-              apply Blocks.WF.mk
+    | (es, ⟨t, t_neq_stmt⟩) =>
+      cases t <;> simp <;> try (apply gwf.inlined_h glt gsig; simpa using wf)
+      · case call h args bret =>
+        if heqg : h ≠ gidx then
+          simp[heqg]
+          apply gwf.inlined_h glt gsig
+          simpa using wf
+        else
+          have heqg := Decidable.of_not_not heqg
+          rw[heqg]
+          simp[heqg] at cspliteq
+          simp
+          let c' : Code :=
+            .merge es (.goto (.mk (bacc.length + (bs.length + gacc.length + 1))
+                                 (args ++ bret.args)))
+          let gacc' := g.inlined_body ((bacc ++ [Block.mk bsig c'] ++ bs ++ gacc).map
+                                          Block.bsig) bret
+          let B := (bacc ++ Block.mk bsig c' :: bs ++ gacc ++ gacc').map (·.bsig)
+          have wf' := wf.blocks.get ⟨bacc.length, by simp⟩
+          simp at wf'
+          have cwf := wf'.code
+          have splitwf := Code.WF.split_wf cwf
+          simp[cspliteq] at splitwf
+          have c'wf : fsigs; B; bsig ⊢ c' WF-code := by
+            simp[c', B]
+            apply Code.WF.merge_wf
+            · exact λ ⟨i, il⟩ => splitwf.1 ⟨i, by simp_all⟩
+            · apply Code.WF.goto
+              apply Cont.WF.mk <;> simp
+              · simp[gacc']
+                have gh := gwf.head.get0eq
+                simp at gh; rw[gh]; simp[BlockSig.inlined, -List.getElem!_eq_getElem?_getD]
+                have req := congrArg BlockSig.r splitwf.2.call_bret.bsig
+                have σeq := congrArg BlockSig.σ splitwf.2.call_bret.bsig
+                rw[getElem!_pos _ bret.b splitwf.2.call_bret.blt]
+                exact gsig ▸ ⟨splitwf.2.call_arity, req, σeq⟩
+              · exact splitwf.2.call_args.append splitwf.2.call_bret.args
+              · match gacc'eq : gacc' with
+                | [] => simp[gacc'] at gacc'eq
+                        simpa[gacc'eq] using gwf.head.headtail
+                | _ :: _ => simp
+          have b'wf : fsigs; B ⊢ ⟨bsig, c'⟩ WF-block := .mk c'wf
+          have wfblocks := wf.blocks
+          have ⟨tmp, gaccwf⟩ := wf.blocks.unappend
+          have ⟨baccwf, tmp'⟩ := tmp.unappend
+          have bswf := tmp'.tail
+          have helper {l : List Block}
+                     (v : IVec (fsigs; ((bacc ++ Block.mk bsig c :: bs ++ gacc).map
+                                          Block.bsig) ⊢ · WF-block) l) :
+                     IVec (Block.WF fsigs ((bacc ++ [Block.mk bsig c'] ++ bs ++
+                                                 (gacc ++ gacc')).map Block.bsig)) l :=
+            v.map (λ b x => by simpa using x.weaken_Bₗ (B' := gacc'.map (·.bsig)))
+          have wf'' : fsigs ⊢ ⟨fsig, bacc ++ [.mk bsig c'] ++
+                                       bs ++ (gacc ++ gacc')⟩ WF-func := by
+            apply Blocks.WF.mk
+            · apply IVec.append
               · apply IVec.append
                 · apply IVec.append
-                  · apply IVec.append
-                    · exact helper baccwf
-                    · apply IVec.singleton
-                      simpa[B] using b'wf
-                  · exact helper bswf
-                · apply IVec.append
-                  · exact helper gaccwf
-                  · simp[gacc']
-                    have x := @inlinedFuncBodyWF fsigs
-                                ((bacc ++ [Block.mk bsig c'] ++ bs ++ gacc).map (·.bsig))
-                                g bret
-                                -- (by have Γeq : (bret.args.length + fsigs[gidx].ret) =
-                                --                (bsig.binds es.length).Γ := by
-                                --       simp[BlockSig.binds]
-                                --       rw[gsig]
-                                --       exact splitwf.2.call_bret.bsig
-                                --     have y : (bacc.map Block.bsig ++ bsig :: (bs.map Block.bsig ++ gacc.map Block.bsig))[bret.b]! = bsig.binds es.length :=
-                                --       getElem!_pos (bacc.map Block.bsig ++ bsig :: (bs.map Block.bsig ++ gacc.map Block.bsig)) bret.b splitwf.2.call_bret.blt ▸
-                                --       splitwf.2.call_bret.bsig ▸
-                                --       Γeq ▸
-                                --       rfl
-                                --     simpa[gsig, y, -List.getElem!_eq_getElem?_getD] using splitwf.2.call_bret)
-                                (bsig.binds es.length).Γ
-                                (by -- have y : (bacc.map Block.bsig ++ bsig :: (bs.map Block.bsig ++ gacc.map Block.bsig))[bret.b]! = bsig.binds es.length :=
-                                    --   getElem!_pos (bacc.map Block.bsig ++ bsig :: (bs.map Block.bsig ++ gacc.map Block.bsig)) bret.b splitwf.2.call_bret.blt ▸
-                                    --   splitwf.2.call_bret.bsig ▸
-                                    --   Γeq ▸
-                                    --   rfl
-                                    have x : (bacc.map Block.bsig ++ ([Block.mk bsig c'].map Block.bsig ++ (bs.map Block.bsig ++ gacc.map Block.bsig))); (bsig.binds es.length) ⊢ bret ( g.fsig.ret ) WF-cont := gsig ▸ splitwf.2.call_bret
-                                    have y : ((bacc ++ ([Block.mk bsig c'] ++ (bs ++ gacc))).map Block.bsig); (bsig.binds es.length) ⊢ bret ( g.fsig.ret ) WF-cont :=
-                                      List.map_append.symm ▸
-                                      List.map_append.symm ▸
-                                      List.map_append.symm ▸
-                                      x
-                                    have bretlt' : bret.b < (List.map Block.bsig (bacc ++ ([Block.mk bsig c'] ++ (bs ++ gacc)))).length := by simpa using splitwf.2.call_bret.blt
-                                    have bretlt'' : bret.b < (bacc ++ ([Block.mk bsig c'] ++ (bs ++ gacc))).length := by simpa using splitwf.2.call_bret.blt
-                                    have z : (bacc ++ ([Block.mk bsig c'] ++ (bs ++ gacc)))[bret.b].bsig = BlockSig.mk (bret.args.length + g.fsig.ret) (bsig.binds es.length).r (bsig.binds es.length).σ := List.getElem_map Block.bsig (h := bretlt') ▸ y.bsig
-                                    have zr : (bacc ++ ([Block.mk bsig c'] ++ (bs ++ gacc)))[bret.b].bsig.r = (bsig.binds es.length).r := congrArg (a₂ := BlockSig.mk (bret.args.length + g.fsig.ret) (bsig.binds es.length).r (bsig.binds es.length).σ) BlockSig.r z
-                                    have zσ : (bacc ++ ([Block.mk bsig c'] ++ (bs ++ gacc)))[bret.b].bsig.σ = (bsig.binds es.length).σ := congrArg (a₂ := BlockSig.mk (bret.args.length + g.fsig.ret) (bsig.binds es.length).r (bsig.binds es.length).σ) BlockSig.σ z
-                                    rw[List.append_assoc]
-                                    rw[List.append_assoc]
-                                    rw[getElem!_pos (List.map (fun x => x.bsig) (bacc ++ ([Block.mk bsig c'] ++ (bs ++ gacc)))) bret.b (by simpa using bretlt')]
-                                    rw[y.bsig]
-                                    simpa using x
-                                )
-                                --(by simpa[gsig, Nat.add_comm] using splitwf.2.call_bret.bsig)
-                                gwf
-                    -- have x := x.unzip.1
-                    have fh : g.blocks.map (extraadd (bacc.map Block.bsig ++ bsig :: (bs.map Block.bsig ++ gacc.map Block.bsig)) bret ∘ Block.bsig) =
-                             g.blocks.map (Block.bsig ∘ inlinedBlock (bacc.map Block.bsig ++ bsig :: (bs.map Block.bsig ++ gacc.map Block.bsig)) (g.blocks.map Block.bsig ) bret) :=
-                      List.map_eq_map_iff.mpr
-                        λ a ain => by simp[extraadd]; cases a.bsig.r <;> simp
-                    simpa[fh, extraadd] using x
-              · have x : IVec (fun b => b.bsig.r.isRetn = true →
-                                       b.bsig.r = ResultSig.retn fsig.ret)
-                             (bacc ++ Block.mk bsig c' :: bs ++ gacc) :=
-                  List.append_cons bacc (Block.mk bsig c') bs ▸
-                  List.append_assoc (bacc ++ [Block.mk bsig c']) bs gacc ▸
-                  (List.append_assoc (bacc ++ [Block.mk bsig c]) bs gacc ▸
-                   List.append_cons bacc (Block.mk bsig c) bs ▸
-                    wf.retns).peephole λ a isretn => (by simp at a isretn; exact a isretn)
-                have z : IVec (fun b => b.bsig.r.isRetn = true →
-                                        b.bsig.r = ResultSig.retn fsig.ret)
-                              (bacc ++ Block.mk bsig c' :: bs ++ gacc ++ gacc') :=
-                  x.append $ by
-                    simp only [gacc', inlinedFuncBody]
-                    apply IVec.from_map_list
-                    intro a isretn
-                    simp[-ResultSig.isExit, -ResultSig.isRetn] at isretn ⊢
-                    cases h : a.bsig.r
-                    · case retn n =>
-                      simp[h] at isretn ⊢
-                      rw[add_retn (bsig := a.bsig) (h ▸ rfl)] at isretn ⊢
-                      simp only [getters] at isretn ⊢
-                      have isretn' : (bacc.map Block.bsig ++ ([Block.mk bsig c].map Block.bsig ++ (bs.map Block.bsig ++ gacc.map Block.bsig)))[bret.b]!.r.isRetn := isretn
-                      have bretlt := splitwf.2.call_bret.blt
-                      have bretlt' : bret.b < (bacc ++ Block.mk bsig c :: bs ++ gacc).length :=
-                        by simpa using bretlt
-                      have x : (bacc ++ ⟨bsig, c⟩ :: bs ++ gacc)[bret.b].bsig.r =
-                               ResultSig.retn fsig.ret :=
-                        wf.retns⁅bret.b⁆ (by
-                          show (bacc ++ Block.mk bsig c :: bs ++ gacc)[bret.b].bsig.r.isRetn = true
-                          rw[← List.map_append, ← List.map_append, ← List.map_append] at isretn'
-                          rw[getElem!_pos (List.map Block.bsig (bacc ++ ([Block.mk bsig c] ++ (bs ++ gacc)))) bret.b (by simpa using bretlt')] at isretn'
-                          rw[List.getElem_map Block.bsig] at isretn'
-                          simpa using isretn')
-                      show (bacc.map Block.bsig ++ ([Block.mk bsig c].map Block.bsig ++
-                             (bs.map Block.bsig ++ gacc.map Block.bsig)))[bret.b]!.r =
-                           ResultSig.retn fsig.ret
-                      rw[← List.map_append, ← List.map_append, ← List.map_append]
-                      rw[getElem!_pos _ bret.b (by simpa using bretlt)]
-                      rw[List.getElem_map]
-                      simpa using x
-                    · case exit n =>
-                      simp[h] at isretn
-                simpa[-ResultSig.isRetn] using z
-              · cases bacc <;> simp <;> simp at wf <;>
-                apply HeadIs.mk <;> simpa using wf.head.get0eq
-            simpa[c', gacc']
-            using @inlinedFuncHWF fsigs fsig g gidx (gacc ++ gacc') bs
-                                  gwf glt gsig (bacc := bacc ++ [.mk bsig c']) wf''
+                  · exact helper baccwf
+                  · apply IVec.singleton
+                    simpa[B] using b'wf
+                · exact helper bswf
+              · apply IVec.append
+                · exact helper gaccwf
+                · simp[gacc']
+                  have x := @gwf.inlined_body fsigs
+                    ((bacc ++ [Block.mk bsig c'] ++ bs ++ gacc).map (·.bsig))
+                    g bret
+                    (bsig.binds es.length).Γ
+                    (by have y : ((bacc++([Block.mk bsig c']++(bs++gacc))).map Block.bsig);
+                                   (bsig.binds es.length) ⊢ bret(g.fsig.ret) WF-cont :=
+                          List.map_append.symm ▸
+                          List.map_append.symm ▸
+                          List.map_append.symm ▸
+                          gsig ▸ splitwf.2.call_bret
+                        have bretlt' : bret.b < ((bacc ++ ([Block.mk bsig c'] ++ (bs ++ gacc))
+                                                  ).map Block.bsig).length :=
+                          by simpa using splitwf.2.call_bret.blt
+                        have bretlt'' : bret.b < (bacc ++ ([Block.mk bsig c'] ++ (bs ++ gacc))
+                                                  ).length :=
+                          by simpa using splitwf.2.call_bret.blt
+                        have z : (bacc ++ ([Block.mk bsig c'] ++ (bs ++ gacc)))[bret.b].bsig =
+                                 BlockSig.mk (bret.args.length + g.fsig.ret)
+                                             (bsig.binds es.length).r
+                                             (bsig.binds es.length).σ :=
+                          List.getElem_map Block.bsig (h := bretlt') ▸
+                          y.bsig
+                        have zr : (bacc ++ ([Block.mk bsig c'] ++ (bs ++ gacc)))[bret.b].bsig.r
+                                  = (bsig.binds es.length).r :=
+                          congrArg (a₂ := BlockSig.mk (bret.args.length + g.fsig.ret)
+                                                      (bsig.binds es.length).r
+                                                      (bsig.binds es.length).σ) BlockSig.r z
+                        have zσ : (bacc ++ ([Block.mk bsig c'] ++ (bs ++ gacc)))[bret.b].bsig.σ
+                                  = (bsig.binds es.length).σ :=
+                          congrArg (a₂ := BlockSig.mk (bret.args.length + g.fsig.ret)
+                                                      (bsig.binds es.length).r
+                                                      (bsig.binds es.length).σ) BlockSig.σ z
+                        rw[List.append_assoc,
+                           List.append_assoc,
+                           getElem!_pos ((bacc ++ ([Block.mk bsig c'] ++ (bs ++ gacc))).map
+                                           Block.bsig) bret.b (by simpa using bretlt'),
+                           y.bsig]
+                        exact y)
+                  have fh : g.blocks.map (BlockSig.inlined (bacc.map Block.bsig ++ bsig ::
+                              (bs.map Block.bsig ++ gacc.map Block.bsig)) bret ∘ Block.bsig) =
+                            g.blocks.map (Block.bsig ∘ Block.inlined (bacc.map Block.bsig ++
+                              bsig :: (bs.map Block.bsig ++ gacc.map Block.bsig))
+                                (g.blocks.map Block.bsig) bret) :=
+                    List.map_eq_map_iff.mpr
+                      λ a ain => by simp[BlockSig.inlined]; cases a.bsig.r <;> simp
+                  simpa[fh, Block.inlined_ext] using x
+            · have x : IVec (fun b => b.bsig.r.isRetn = true →
+                                     b.bsig.r = ResultSig.retn fsig.ret)
+                           (bacc ++ Block.mk bsig c' :: bs ++ gacc) :=
+                List.append_cons bacc (Block.mk bsig c') bs ▸
+                List.append_assoc (bacc ++ [Block.mk bsig c']) bs gacc ▸
+                (List.append_assoc (bacc ++ [Block.mk bsig c]) bs gacc ▸
+                 List.append_cons bacc (Block.mk bsig c) bs ▸
+                  wf.retns).peephole λ a isretn => (by simp at a isretn; exact a isretn)
+              have z : IVec (fun b => b.bsig.r.isRetn = true →
+                                      b.bsig.r = ResultSig.retn fsig.ret)
+                            (bacc ++ Block.mk bsig c' :: bs ++ gacc ++ gacc') :=
+                x.append $ by
+                  simp only [gacc', Func.inlined_body]
+                  apply IVec.from_map_list
+                  intro a isretn
+                  simp[-ResultSig.isExit, -ResultSig.isRetn] at isretn ⊢
+                  cases h : a.bsig.r
+                  · case retn n =>
+                    simp[h] at isretn ⊢
+                    rw[a.bsig.inlined_retn (h ▸ rfl)] at isretn ⊢
+                    simp only [getters] at isretn ⊢
+                    have isretn' : (bacc.map Block.bsig ++ ([Block.mk bsig c].map Block.bsig ++
+                                     (bs.map Block.bsig ++ gacc.map Block.bsig))
+                                     )[bret.b]!.r.isRetn := isretn
+                    have bretlt := splitwf.2.call_bret.blt
+                    have bretlt' : bret.b < (bacc ++ Block.mk bsig c :: bs ++ gacc).length :=
+                      by simpa using bretlt
+                    have x : (bacc ++ ⟨bsig, c⟩ :: bs ++ gacc)[bret.b].bsig.r =
+                             ResultSig.retn fsig.ret :=
+                      wf.retns⁅bret.b⁆ (by
+                        show (bacc ++ Block.mk bsig c :: bs ++ gacc)[bret.b].bsig.r.isRetn
+                        rw[← List.map_append, ← List.map_append, ← List.map_append] at isretn'
+                        rw[getElem!_pos (List.map Block.bsig (bacc ++ ([Block.mk bsig c] ++
+                             (bs ++ gacc)))) bret.b (by simpa using bretlt')] at isretn'
+                        rw[List.getElem_map Block.bsig] at isretn'
+                        simpa using isretn')
+                    show (bacc.map Block.bsig ++ ([Block.mk bsig c].map Block.bsig ++
+                           (bs.map Block.bsig ++ gacc.map Block.bsig)))[bret.b]!.r =
+                         ResultSig.retn fsig.ret
+                    rw[← List.map_append, ← List.map_append, ← List.map_append]
+                    rw[getElem!_pos _ bret.b (by simpa using bretlt)]
+                    rw[List.getElem_map]
+                    simpa using x
+                  · case exit n =>
+                    simp[h] at isretn
+              simpa[-ResultSig.isRetn] using z
+            · cases bacc <;> simp <;> simp at wf <;>
+              apply HeadIs.mk <;> simpa using wf.head.get0eq
+          simpa[c', gacc']
+          using @gwf.inlined_h fsigs fsig g gidx (gacc ++ gacc') bs
+                                  glt gsig (bacc := bacc ++ [.mk bsig c']) wf''
 
 /--
 Inline each call to g in the body of f
 -/
-def inlinedFunc (f g : Func) (gidx : FuncIdx) : Func :=
-  .mk f.fsig (inlinedFuncH g gidx [] f.blocks [])
+def Func.inline (f g : Func) (gidx : FuncIdx) : Func :=
+  .mk f.fsig (g.inlined_h gidx [] f.blocks [])
 
-theorem inlinedFuncWF {fsigs} {f g : Func} {gidx : FuncIdx}
-                      (gwf : fsigs ⊢ g WF-func) (glt : gidx < fsigs.length)
-                      (gsig : fsigs[gidx] = g.fsig) (wf : fsigs ⊢ f WF-func) :
-                      fsigs ⊢ inlinedFunc f g gidx WF-func :=
-  inlinedFuncHWF gwf glt gsig ((List.append_nil f.blocks).symm ▸ wf)
+/--
+Inlining a function in the body of another preserves well-formedness
+-/
+theorem Func.WF.inline
+    {fsigs f g gidx}
+    (glt : gidx < fsigs.length)
+    (gsig : fsigs[gidx] = g.fsig)
+    (fwf : fsigs ⊢ f WF-func)
+    (gwf : fsigs ⊢ g WF-func) :
+    fsigs ⊢ f.inline g gidx WF-func :=
+  gwf.inlined_h glt gsig ((List.append_nil f.blocks).symm ▸ fwf)
 
-namespace Program
-  def inlineCallsInFunc : (P : Program) -> (fidx gidx : FuncIdx) -> (g : Func) -> Program
-    | .mk funs, fidx, gidx, g =>
-      .mk (funs.mapIdx (λ i f => if i = fidx then inlinedFunc f g gidx else f))
-
-  def inlineCalls : (P : Program) -> (gidx : FuncIdx) -> (g : Func) -> Program
-    | .mk funs, gidx, g => .mk (funs.mapIdx (λ i f => if i = gidx then f else inlinedFunc f g gidx))
-
-end Program
