SporkProofs/ParReduce.lean
@@ -2,57 +2,91 @@ import SporkProofs.Syntax
 import SporkProofs.Notation
 import SporkProofs.WFSyntax
 
-def fibExample: Program :=
-  PROGRAM (
-    func main(
-      block start() {n ← 10, CALL fib(n) ⊳ goto ret()},
-      block ret(r) {RETURN(r)}
-    ),
-    func fib(
-      block start(n) {SPORK (goto body(n), goto spwn(n))},
-      block body(n) {n₁ ← n - 1, CALL fib(n₁) ⊳ goto cont(n)},
-      block cont(n, r₁) {SPOIN (goto unpr(n, r₁), goto prom(r₁))},
-      block unpr(n, r₁) {n₂ ← n - 2, CALL fib(n₂) ⊳ goto ret(r₁)},
-      block prom(r₁, r₂) {GOTO ret(r₁,r₂)},
-      block ret(r₁, r₂) {r ← r₁ + r₂, RETURN(r)},
-      block spwn(n) {n₂ ← n - 2, CALL fib(n₂) ⊳ goto exit()},
-      block exit(r₂) {RETURN(r₂)}
-    )
+/-!
+Implementation of `par` and `reduce` in Spork IR,
+along with proofs of their well-formedness.
+
+We use the DSL notation for Spork IR defined in `SporkProofs.Notation`
+-/
+
+
+def par (f g : FuncIdx) : Func := func (
+    block start():
+      SPORK (goto body(), goto spwn())
+    block body():
+      CALL f() ⊳ goto cont()
+    block cont(a):
+      SPOIN (goto unpr(a), goto prom(a))
+    block unpr(a):
+      CALL g() ⊳ goto ret(a)
+    block prom(r₁, r₂):
+      GOTO ret(r₁,r₂)
+    block ret(a, b):
+      RETURN(a,b)
+    block spwn():
+      CALL g() ⊳ goto exit()
+    block exit(b):
+      RETURN(b)
   )
 
-def parExample (f g : FuncIdx) : Func := func (
-    block start() {SPORK (goto body(), goto spwn())},
-    block body() {CALL f() ⊳ goto cont()},
-    block cont(a) {SPOIN (goto unpr(a), goto prom(a))},
-    block unpr(a) {CALL g() ⊳ goto ret(a)},
-    block prom(r₁, r₂) {GOTO ret(r₁,r₂)},
-    block ret(a, b) {RETURN(a,b)},
-    block spwn() {CALL g() ⊳ goto exit()},
-    block exit(b) {RETURN(b)}
+def reduce (f c reduce : FuncIdx) : Func := func (
+    block start(z,a,i,j):
+      GOTO guard(z,i,j,a)
+    block guard(z,i,j,a):
+      b ← i >= j,
+      IF b THEN goto done(a) ELSE goto iter(z,i,j,a)
+    block done(a):
+      RETURN(a)
+    block iter(z,i,j,a):
+      SPORK (goto body(z,i,j,a), goto split(z,i,j,a))
+    block body(z,i,j,a):
+      CALL f(i) ⊳ goto accum(z,i,j,a)
+    block accum(z,i,j,a,a₁):
+      CALL c(a,a₁) ⊳ goto cont(z,i,j)
+    block cont(z,i,j,a):
+      SPOIN (goto next(z,i,j,a), goto brk(a))
+    block next(z,i,j,a):
+      i₁ ← i + 1,
+      GOTO guard(z,i₁,j,a)
+    block brk(a,a₁):
+      CALL c(a,a₁) ⊳ goto done()
+    block split(z,i,j,a):
+      i₁ ← i + 1,
+      k ← i₁ + j,
+      m ← k / 2,
+      SPORK (goto left(z,i₁,m,j), goto right(z,m,j))
+    block left(z,i,m,j):
+      CALL reduce(z,z,i,m) ⊳ goto middle(z,m,j)
+    block middle(z,m,j,a):
+      SPOIN(goto leftover(z,m,j,a), goto merge(a))
+    block leftover(z,m,j,a):
+      CALL reduce(z,a,m,j) ⊳ goto exit()
+    block merge(a,a₁):
+      CALL c(a,a₁) ⊳ goto exit()
+    block exit(a):
+      RETURN(a)
+    block right(z,m,j):
+      CALL reduce(z,z,m,j) ⊳ goto exit()
   )
 
-theorem parExampleWF : [⟨0, 1⟩, ⟨0, 1⟩] ⊢ (parExample 0 1) WF-func :=
+/--
+  [⟨0, 1⟩, ⟨0, 1⟩] => [f takes 0 args and returns 1, g takes 0 args and returns 1]
+  par 0 1 => par (func idx 0 = f, func idx 1 = g)
+-/
+theorem parWF : [⟨0, 1⟩, ⟨0, 1⟩] ⊢ (par 0 1) WF-func :=
   by decide
 
-def reduceExample (f c reduce : FuncIdx) : Func := func (
-    block start(z,a,i,j) {GOTO guard(z,i,j,a)},
-    block guard(z,i,j,a) {b ← i >= j, IF b THEN goto done(a) ELSE goto iter(z,i,j,a)},
-    block done(a) {RETURN(a)},
-    block iter(z,i,j,a) {SPORK (goto body(z,i,j,a), goto split(z,i,j,a))},
-    block body(z,i,j,a) {CALL f(i) ⊳ goto accum(z,i,j,a)},
-    block accum(z,i,j,a,a₁) {CALL c(a,a₁) ⊳ goto cont(z,i,j)},
-    block cont(z,i,j,a) {SPOIN (goto next(z,i,j,a), goto brk(a))},
-    block next(z,i,j,a) {i₁ ← i + 1, GOTO guard(z,i₁,j,a)},
-    block brk(a,a₁) {CALL c(a,a₁) ⊳ goto done()},
-    block split(z,i,j,a) {i₁ ← i + 1, k ← i₁ + j, m ← k / 2, SPORK (goto left(z,i₁,m,j), goto right(z,m,j))},
-    block left(z,i,m,j) {CALL reduce(z,z,i,m) ⊳ goto middle(z,m,j)},
-    block middle(z,m,j,a) {SPOIN(goto leftover(z,m,j,a), goto merge(a))},
-    block leftover(z,m,j,a) {CALL reduce(z,a,m,j) ⊳ goto exit()},
-    block merge(a,a₁) {CALL c(a,a₁) ⊳ goto exit()},
-    block exit(a) {RETURN(a)},
-    block right(z,m,j) {CALL reduce(z,z,m,j) ⊳ goto exit()}
-  )
+/--
+[⟨1, 1⟩, ⟨2, 1⟩, ⟨4, 1⟩] =>
+  [f takes 1 arg and returns 1,
+   c(ombine) takes 2 args and returns 1,
+   reduce (needed for recursive calls) takes 4 args and returns 1]
 
--- set_option maxRecDepth 10000
-theorem reduceExampleWF : [⟨1, 1⟩, ⟨2, 1⟩, ⟨4, 1⟩] ⊢ (reduceExample 0 1 2) WF-func :=
-  by simp[reduceExample, Nat.repeat]; decide
+reduce 0 1 2 => reduce (func idx 0 = f, func idx 1 = c, func idx 2 = reduce)
+
+this nearly reaches the default max recursion depth,
+if you get an error about it, increase the limit:
+`set_option maxRecDepth 10000`
+-/
+theorem reduceWF : [⟨1, 1⟩, ⟨2, 1⟩, ⟨4, 1⟩] ⊢ (reduce 0 1 2) WF-func :=
+  by simp[reduce, Nat.repeat]; decide
